---
title: Summation LaTeX Equations
description: LaTeX of the summation expression
layout: post
toc: true
comments: true
categories: [math, latex]
---


$$
\sum_{i=m}^n a_i = a_m + a_{m + 1} + a_{m + 2} + \dots + a_{n - 1} + a_n \\
$$

```text
\sum_{i=m}^n a_i = a_m + a_{m + 1} + a_{m + 2} + \dots + a_{n - 1} + a_n \\
```

$$
\begin{align*}
\sum_{i=m}^n ca_i &= c \sum_{i=m}^n a_i \\
\sum_{i=m}^n (a_i + b_i) &= c \sum_{i=m}^n a_i + c \sum_{i=m}^n b_i \\
\sum_{i=m}^n (a_i - b_i) &= c \sum_{i=m}^n a_i - c \sum_{i=m}^n b_i
\end{align*}
$$

```text
\sum_{i=m}^n ca_i &= c \sum_{i=m}^n a_i \\
\sum_{i=m}^n (a_i + b_i) &= c \sum_{i=m}^n a_i + c \sum_{i=m}^n b_i \\
\sum_{i=m}^n (a_i - b_i) &= c \sum_{i=m}^n a_i - c \sum_{i=m}^n b_i
```

$$
\begin{align*}
\sum_{i=1}^n 1 &= n \\
\sum_{i=1}^n c &= nc \\
\sum_{i=1}^n i &= \frac{n(n + 1)}{2} \\
\sum_{i=1}^n i^2 &= \frac{n(n + 1)(2n + 1)}{6} \\
\sum_{i=1}^n i^3 &= [\frac{n(n + 1)}{2}]^2
\end{align*}
$$

```text
\sum_{i=1}^n 1 &= n \\
\sum_{i=1}^n c &= nc \\
\sum_{i=1}^n i &= \frac{n(n + 1)}{2} \\
\sum_{i=1}^n i^2 &= \frac{n(n + 1)(2n + 1)}{6} \\
\sum_{i=1}^n i^3 &= [\frac{n(n + 1)}{2}]^2
```
